update simulate layer to v103

RocqOfRust/revm/revm_interpreter/instructions/simulate/host/sstore.v
@@ -40,8 +40,10 @@ Definition sstore
   let spec_id :=
     IInterpreterTypes.(InterpreterTypes.RuntimeFlag_for_RuntimeFlag).(RuntimeFlag.spec_id)
       interpreter.(Interpreter.runtime_flag) in
-  if (Impl_SpecId.is_enabled_in spec_id SpecId.ISTANBUL)
-      && (i[Impl_Gas.remaining interpreter.(Interpreter.gas)] <=? i[constants.CALL_STIPEND]) then
+  if (Bool.eqb (Impl_SpecId.is_enabled_in spec_id SpecId.ISTANBUL) true)
+      && (Bool.eqb
+        (i[Impl_Gas.remaining interpreter.(Interpreter.gas)] <=? i[constants.CALL_STIPEND])
+        true) then
     (halt interpreter instruction_result.InstructionResult.ReentrancySentryOOG, host)
   else
   gas_macro interpreter
@@ -116,4 +118,1023 @@ Lemma sstore_eq
     )
   }}.
 Proof.
-Admitted.
+  intros.
+  subst result.
+  with_strategy transparent [run_sstore] unfold sstore, run_sstore; cbn.
+  require_non_staticcall_macro_eq InterpreterTypesEq.
+  popn_macro_eq InterpreterTypesEq.
+  match goal with
+  | arr : array.t aliases.U256.t _ |- _ =>
+    destruct arr as [[index [value []]]]
+  end.
+  s. {
+    apply InterpreterTypesEq.
+  }
+  s. {
+    apply InterpreterTypesEq.
+  }
+  s. {
+    apply InterpreterTypesEq.
+  }
+  s. {
+    apply Impl_SpecId.is_enabled_in_eq.
+  }
+  destruct
+    (Bool.eqb
+      (Impl_SpecId.is_enabled_in
+      (IInterpreterTypes.(InterpreterTypes.RuntimeFlag_for_RuntimeFlag)
+        .(RuntimeFlag.spec_id) interpreter.(Interpreter.runtime_flag))
+      SpecId.ISTANBUL)
+      true) eqn:H_istanbul; cbn.
+  - eapply Run.Call
+      with
+        (output_inter := true)
+        (stack_inter :=
+          [interpreter<|Interpreter.stack := s|>; host; tt;
+           IInterpreterTypes.(InterpreterTypes.InputsTrait_for_Input)
+             .(InputTraits.target_address) interpreter.(Interpreter.input);
+           IInterpreterTypes.(InterpreterTypes.RuntimeFlag_for_RuntimeFlag)
+             .(RuntimeFlag.spec_id) interpreter.(Interpreter.runtime_flag)]%stack).
+    {
+      apply Run.PureEq.
+      cbn.
+      repeat f_equal.
+      exact H_istanbul.
+    }
+    cbn.
+    eapply Run.Call. {
+      apply Impl_Gas.remaining_interpreter_eq.
+    }
+    cbn.
+    eapply Run.Call. {
+      apply CALL_STIPEND_eq.
+    }
+    cbn.
+    eapply Run.Call. {
+      apply Run.Pure.
+    }
+    cbn.
+    destruct
+      (Bool.eqb
+        (i[Impl_Gas.remaining interpreter.(Interpreter.gas)] <=? i[constants.CALL_STIPEND])
+        true) eqn:H_stipend; cbn.
+    + eapply Run.Call
+        with
+          (output_inter := true)
+          (stack_inter :=
+            [interpreter<|Interpreter.stack := s|>; host; tt;
+             IInterpreterTypes.(InterpreterTypes.InputsTrait_for_Input)
+               .(InputTraits.target_address) interpreter.(Interpreter.input);
+             IInterpreterTypes.(InterpreterTypes.RuntimeFlag_for_RuntimeFlag)
+               .(RuntimeFlag.spec_id) interpreter.(Interpreter.runtime_flag)]%stack).
+      {
+        apply Run.PureEq.
+        cbn.
+        repeat f_equal.
+        exact H_stipend.
+      }
+      cbn.
+      s. {
+        eapply halt_eq;
+        exact InterpreterTypesEq.
+      }
+      cbn.
+      unfold sstore.
+      cbn.
+      replace
+        (Bool.eqb
+          (Impl_SpecId.is_enabled_in
+          (IInterpreterTypes.(InterpreterTypes.RuntimeFlag_for_RuntimeFlag)
+            .(RuntimeFlag.spec_id) interpreter.(Interpreter.runtime_flag))
+          SpecId.ISTANBUL)
+        true)
+        with true by (symmetry; exact H_istanbul).
+      cbn.
+      replace
+        (Bool.eqb
+          (i[Impl_Gas.remaining interpreter.(Interpreter.gas)] <=? i[constants.CALL_STIPEND])
+          true)
+        with true by (symmetry; exact H_stipend).
+      cbn.
+      apply Run.PureEq.
+      cbn.
+      setoid_rewrite H_istanbul.
+      setoid_rewrite H_stipend.
+      cbn.
+      reflexivity.
+    + eapply Run.Call
+        with
+          (output_inter := false)
+          (stack_inter :=
+            [interpreter<|Interpreter.stack := s|>; host; tt;
+             IInterpreterTypes.(InterpreterTypes.InputsTrait_for_Input)
+               .(InputTraits.target_address) interpreter.(Interpreter.input);
+             IInterpreterTypes.(InterpreterTypes.RuntimeFlag_for_RuntimeFlag)
+               .(RuntimeFlag.spec_id) interpreter.(Interpreter.runtime_flag)]%stack).
+      {
+        apply Run.PureEq.
+        cbn.
+        repeat f_equal.
+        exact H_stipend.
+      }
+      cbn.
+      s. {
+        apply InterpreterTypesEq.
+      }
+      eapply Run.Call. {
+        apply calc.static_sstore_cost_eq.
+      }
+      cbn.
+      s. {
+        apply Impl_Gas.record_cost_interpreter_eq.
+      }
+      destruct
+        (Impl_Gas.record_cost
+          interpreter.(Interpreter.gas)
+          (calc.static_sstore_cost
+            (IInterpreterTypes.(InterpreterTypes.RuntimeFlag_for_RuntimeFlag)
+              .(RuntimeFlag.spec_id) interpreter.(Interpreter.runtime_flag)))
+        ) as [gas_after_static|] eqn:H_static_gas; cbn.
+      * eapply Run.Call
+          with
+            (output_inter := false)
+            (stack_inter :=
+              [interpreter<|Interpreter.stack := s|><|Interpreter.gas := gas_after_static|>;
+               host; tt;
+               IInterpreterTypes.(InterpreterTypes.InputsTrait_for_Input)
+                 .(InputTraits.target_address) interpreter.(Interpreter.input);
+               IInterpreterTypes.(InterpreterTypes.RuntimeFlag_for_RuntimeFlag)
+                 .(RuntimeFlag.spec_id) interpreter.(Interpreter.runtime_flag);
+               tt]%stack).
+        {
+          apply Run.PureEq.
+          cbn.
+          setoid_rewrite H_static_gas.
+          cbn.
+          reflexivity.
+        }
+        cbn.
+        eapply Run.Call
+          with
+            (output_inter := false)
+            (stack_inter :=
+              [interpreter<|Interpreter.stack := s|><|Interpreter.gas := gas_after_static|>;
+               host; tt;
+               IInterpreterTypes.(InterpreterTypes.InputsTrait_for_Input)
+                 .(InputTraits.target_address) interpreter.(Interpreter.input);
+               IInterpreterTypes.(InterpreterTypes.RuntimeFlag_for_RuntimeFlag)
+                 .(RuntimeFlag.spec_id) interpreter.(Interpreter.runtime_flag);
+               tt]%stack).
+        {
+          apply Run.Pure.
+        }
+        cbn.
+        apply Run.LetUnfold.
+        cbn.
+        get_can_access.
+        cbn.
+        eapply Run.Call. {
+          apply Impl_SpecId.is_enabled_in_eq.
+        }
+        cbn.
+        destruct
+          (Impl_SpecId.is_enabled_in
+            (IInterpreterTypes.(InterpreterTypes.RuntimeFlag_for_RuntimeFlag)
+              .(RuntimeFlag.spec_id) interpreter.(Interpreter.runtime_flag))
+            SpecId.BERLIN) eqn:H_berlin; cbn.
+        -- eapply Run.Call
+             with
+               (output_inter := true)
+               (stack_inter :=
+                 [interpreter<|Interpreter.stack := s|><|Interpreter.gas := gas_after_static|>;
+                  host; tt;
+                  IInterpreterTypes.(InterpreterTypes.InputsTrait_for_Input)
+                    .(InputTraits.target_address) interpreter.(Interpreter.input);
+                  IInterpreterTypes.(InterpreterTypes.RuntimeFlag_for_RuntimeFlag)
+                    .(RuntimeFlag.spec_id) interpreter.(Interpreter.runtime_flag);
+                  tt; tt]%stack).
+           {
+             apply Run.PureEq.
+             cbn.
+             repeat f_equal.
+	           }
+	           cbn.
+	           apply Run.LetUnfold.
+	           cbn.
+	           eapply Run.Call. {
+	             apply Impl_Gas.remaining_interpreter_eq.
+	           }
+	           cbn.
+	           eapply Run.Call. {
+	             apply COLD_SLOAD_COST_ADDITIONAL_eq.
+	           }
+	           cbn.
+		           eapply Run.Call. {
+		             apply Run.Pure.
+		           }
+		           cbn.
+			           apply Run.LetUnfold.
+			           cbn.
+			           get_can_access.
+			           cbn.
+			           get_can_access.
+			           cbn.
+			           eapply Run.Call. {
+			             apply HostEq.
+			           }
+		           destruct
+		             (IHost.(Host.sstore_skip_cold_load) host
+		               (IInterpreterTypes.(InterpreterTypes.InputsTrait_for_Input)
+		                 .(InputTraits.target_address) interpreter.(Interpreter.input))
+		               index value
+		               (i[Impl_Gas.remaining gas_after_static] <? (2100 - 100) mod 2 ^ 64))
+		             as [[state_load|load_error] host_after] eqn:H_sstore_result;
+		             cbn.
+	           ++ get_can_access.
+	              cbn.
+	              setoid_rewrite H_sstore_result.
+	              cbn.
+	              s. {
+	                apply InterpreterTypesEq.
+	              }
+	              get_can_access.
+	              cbn.
+	              eapply Run.Call. {
+	                apply calc.dyn_sstore_cost_eq.
+	              }
+	              cbn.
+	              s. {
+	                apply Impl_Gas.record_cost_interpreter_eq.
+	              }
+	              match goal with
+	              | |- context[Impl_Gas.record_cost ?gas ?cost] =>
+	                  destruct (Impl_Gas.record_cost gas cost)
+	                    as [gas_after_dynamic|] eqn:H_dynamic_gas
+	              end;
+	              cbn.
+	              ** eapply Run.Call. {
+	                   apply Run.Pure.
+	                 }
+	                 cbn.
+	                 eapply Run.Call. {
+	                   apply Run.Pure.
+	                 }
+	                 cbn.
+	                 apply Run.LetUnfold.
+	                 cbn.
+	                 s. {
+	                   apply InterpreterTypesEq.
+	                 }
+	                 eapply Run.Call. {
+	                   apply calc.sstore_refund_eq.
+	                 }
+		                 cbn.
+		                 s. {
+		                   apply Impl_Gas.record_refund_interpreter_eq.
+		                 }
+		                 cbn.
+		                 apply Run.PureEq.
+	                 cbn.
+	                 setoid_rewrite H_istanbul.
+	                 cbn.
+	                 setoid_rewrite H_stipend.
+	                 cbn.
+	                 unfold gas_macro.
+	                 cbn.
+	                 setoid_rewrite H_static_gas.
+	                 cbn.
+	                 symmetry in H_berlin.
+	                 destruct H_berlin.
+	                 cbn.
+	                 setoid_rewrite H_sstore_result.
+	                 cbn.
+	                 unfold gas_macro.
+	                 cbn.
+	                 unfold calc.dyn_sstore_cost in H_dynamic_gas.
+	                 unfold calc.sstore_cost in H_dynamic_gas.
+	                 cbn in H_dynamic_gas.
+	                 unfold calc.dyn_sstore_cost.
+	                 unfold calc.sstore_cost.
+	                 cbn.
+	                 setoid_rewrite H_dynamic_gas.
+	                 cbn.
+	                 unfold calc.sstore_refund.
+	                 cbn.
+	                 reflexivity.
+	              ** s. {
+	                   eapply halt_oog_eq;
+	                   exact InterpreterTypesEq.
+	                 }
+	                 cbn.
+	                 apply Run.PureEq.
+	                 cbn.
+	                 setoid_rewrite H_istanbul.
+	                 cbn.
+	                 setoid_rewrite H_stipend.
+	                 cbn.
+	                 unfold gas_macro.
+	                 cbn.
+	                 setoid_rewrite H_static_gas.
+	                 cbn.
+	                 setoid_rewrite H_sstore_result.
+	                 cbn.
+	                 unfold gas_macro.
+	                 cbn.
+	                 setoid_rewrite H_dynamic_gas.
+	                 cbn.
+	                 symmetry in H_berlin.
+	                 destruct H_berlin.
+	                 cbn.
+	                 reflexivity.
+		           ++ destruct load_error; cbn.
+		              ** get_can_access.
+		                 cbn.
+		                 setoid_rewrite H_sstore_result.
+		                 cbn.
+		                 get_can_access.
+		                 cbn.
+		                 setoid_rewrite H_sstore_result.
+		                 cbn.
+		                 setoid_rewrite H_sstore_result.
+		                 cbn.
+			                 s. {
+			                   eapply halt_fatal_eq;
+			                   exact InterpreterTypesEq.
+			                 }
+			                 cbn.
+			                 apply Run.PureEq.
+			                 cbn.
+			                 setoid_rewrite H_istanbul.
+			                 cbn.
+			                 setoid_rewrite H_stipend.
+			                 cbn.
+			                 unfold gas_macro.
+			                 cbn.
+			                 setoid_rewrite H_static_gas.
+			                 cbn.
+			                 setoid_rewrite H_sstore_result.
+			                 cbn.
+			                 symmetry in H_berlin.
+			                 destruct H_berlin.
+			                 cbn.
+			                 reflexivity.
+		              ** get_can_access.
+		                 cbn.
+		                 setoid_rewrite H_sstore_result.
+		                 cbn.
+		                 get_can_access.
+		                 cbn.
+		                 setoid_rewrite H_sstore_result.
+		                 cbn.
+		                 s. {
+		                   eapply halt_oog_eq;
+		                   exact InterpreterTypesEq.
+		                 }
+		                 cbn.
+			                 apply Run.PureEq.
+			                 cbn.
+			                 setoid_rewrite H_istanbul.
+			                 cbn.
+			                 setoid_rewrite H_stipend.
+			                 cbn.
+			                 unfold gas_macro.
+			                 cbn.
+			                 setoid_rewrite H_static_gas.
+			                 cbn.
+			                 setoid_rewrite H_sstore_result.
+			                 cbn.
+			                 symmetry in H_berlin.
+			                 destruct H_berlin.
+			                 cbn.
+			                 reflexivity.
+	        -- eapply Run.Call
+	             with
+	               (output_inter := false)
+	               (stack_inter :=
+	                 [interpreter<|Interpreter.stack := s|><|Interpreter.gas := gas_after_static|>;
+	                  host; tt;
+	                  IInterpreterTypes.(InterpreterTypes.InputsTrait_for_Input)
+	                    .(InputTraits.target_address) interpreter.(Interpreter.input);
+	                  IInterpreterTypes.(InterpreterTypes.RuntimeFlag_for_RuntimeFlag)
+	                    .(RuntimeFlag.spec_id) interpreter.(Interpreter.runtime_flag);
+	                  tt; tt]%stack).
+		           {
+		             apply Run.PureEq.
+		             cbn.
+		             repeat f_equal.
+		           }
+		           cbn.
+		           get_can_access.
+		           cbn.
+		           eapply Run.Call. {
+		             apply HostEq.
+		           }
+		           destruct
+			             (IHost.(Host.sstore) host
+			               (IInterpreterTypes.(InterpreterTypes.InputsTrait_for_Input)
+			                 .(InputTraits.target_address) interpreter.(Interpreter.input))
+			               index value)
+			             as [[state_load|] host_after] eqn:H_sstore_result;
+			             cbn.
+	           ++ s. {
+	                apply InterpreterTypesEq.
+	              }
+	              get_can_access.
+	              cbn.
+	              eapply Run.Call. {
+	                apply calc.dyn_sstore_cost_eq.
+	              }
+	              cbn.
+	              s. {
+	                apply Impl_Gas.record_cost_interpreter_eq.
+	              }
+	              match goal with
+	              | |- context[Impl_Gas.record_cost ?gas ?cost] =>
+	                  destruct (Impl_Gas.record_cost gas cost)
+	                    as [gas_after_dynamic|] eqn:H_dynamic_gas
+	              end;
+	              cbn.
+	              ** eapply Run.Call. {
+	                   apply Run.Pure.
+	                 }
+	                 cbn.
+	                 eapply Run.Call. {
+	                   apply Run.Pure.
+	                 }
+	                 cbn.
+	                 apply Run.LetUnfold.
+	                 cbn.
+	                 s. {
+	                   apply InterpreterTypesEq.
+	                 }
+	                 eapply Run.Call. {
+	                   apply calc.sstore_refund_eq.
+	                 }
+	                 cbn.
+	                 s. {
+	                   apply Impl_Gas.record_refund_interpreter_eq.
+	                 }
+	                 cbn.
+	                 apply Run.PureEq.
+	                 cbn.
+	                 setoid_rewrite H_istanbul.
+	                 cbn.
+	                 setoid_rewrite H_stipend.
+	                 cbn.
+	                 unfold gas_macro.
+	                 cbn.
+	                 setoid_rewrite H_static_gas.
+	                 cbn.
+	                 symmetry in H_berlin.
+	                 destruct H_berlin.
+	                 cbn.
+	                 setoid_rewrite H_sstore_result.
+	                 cbn.
+	                 unfold gas_macro.
+	                 cbn.
+	                 unfold calc.dyn_sstore_cost in H_dynamic_gas.
+	                 unfold calc.sstore_cost in H_dynamic_gas.
+	                 cbn in H_dynamic_gas.
+	                 unfold calc.dyn_sstore_cost.
+	                 unfold calc.sstore_cost.
+	                 cbn.
+	                 setoid_rewrite H_dynamic_gas.
+	                 cbn.
+	                 unfold calc.sstore_refund.
+	                 cbn.
+	                 reflexivity.
+	              ** s. {
+	                   eapply halt_oog_eq;
+	                   exact InterpreterTypesEq.
+	                 }
+	                 cbn.
+	                 apply Run.PureEq.
+	                 cbn.
+	                 setoid_rewrite H_istanbul.
+	                 cbn.
+	                 setoid_rewrite H_stipend.
+	                 cbn.
+	                 unfold gas_macro.
+	                 cbn.
+	                 setoid_rewrite H_static_gas.
+	                 cbn.
+	                 symmetry in H_berlin.
+	                 destruct H_berlin.
+	                 cbn.
+	                 setoid_rewrite H_sstore_result.
+	                 cbn.
+	                 unfold gas_macro.
+	                 cbn.
+	                 unfold calc.dyn_sstore_cost in H_dynamic_gas.
+	                 unfold calc.sstore_cost in H_dynamic_gas.
+	                 cbn in H_dynamic_gas.
+	                 unfold calc.dyn_sstore_cost.
+	                 unfold calc.sstore_cost.
+	                 cbn.
+	                 setoid_rewrite H_dynamic_gas.
+	                 cbn.
+	                 reflexivity.
+		           ++ s. {
+	                eapply halt_fatal_eq;
+	                exact InterpreterTypesEq.
+	              }
+	              cbn.
+	              apply Run.PureEq.
+	              cbn.
+	              setoid_rewrite H_istanbul.
+	              cbn.
+	              setoid_rewrite H_stipend.
+	              cbn.
+	              unfold gas_macro.
+	              cbn.
+	              setoid_rewrite H_static_gas.
+	              cbn.
+	              symmetry in H_berlin.
+	              destruct H_berlin.
+		              cbn.
+		              setoid_rewrite H_sstore_result.
+		              cbn.
+		              reflexivity.
+      * eapply Run.Call. {
+          apply Run.Pure.
+        }
+        cbn.
+        eapply Run.Call. {
+          apply Run.Pure.
+        }
+        cbn.
+        setoid_rewrite H_static_gas.
+        cbn.
+        apply Run.LetUnfold.
+        cbn.
+        eapply Run.Call. {
+          eapply halt_oog_eq;
+          exact InterpreterTypesEq.
+        }
+        cbn.
+        unfold sstore.
+        cbn.
+        setoid_rewrite H_istanbul.
+        setoid_rewrite H_stipend.
+        cbn.
+        unfold gas_macro.
+        cbn.
+        apply Run.PureEq.
+        cbn.
+        setoid_rewrite H_static_gas.
+        cbn.
+        reflexivity.
+  - eapply Run.Call
+      with
+        (output_inter := false)
+        (stack_inter :=
+          [interpreter<|Interpreter.stack := s|>; host; tt;
+           IInterpreterTypes.(InterpreterTypes.InputsTrait_for_Input)
+             .(InputTraits.target_address) interpreter.(Interpreter.input);
+           IInterpreterTypes.(InterpreterTypes.RuntimeFlag_for_RuntimeFlag)
+             .(RuntimeFlag.spec_id) interpreter.(Interpreter.runtime_flag)]%stack).
+    {
+      apply Run.PureEq.
+      cbn.
+      repeat f_equal.
+      exact H_istanbul.
+	    }
+	    cbn.
+	    s. {
+	      apply InterpreterTypesEq.
+	    }
+	    eapply Run.Call. {
+	      apply calc.static_sstore_cost_eq.
+	    }
+	    cbn.
+	    s. {
+	      apply Impl_Gas.record_cost_interpreter_eq.
+	    }
+	    destruct
+	      (Impl_Gas.record_cost
+	        interpreter.(Interpreter.gas)
+	        (calc.static_sstore_cost
+	          (IInterpreterTypes.(InterpreterTypes.RuntimeFlag_for_RuntimeFlag)
+	            .(RuntimeFlag.spec_id) interpreter.(Interpreter.runtime_flag)))
+	      ) as [gas_after_static|] eqn:H_static_gas; cbn.
+	    + eapply Run.Call
+	        with
+	          (output_inter := false)
+	          (stack_inter :=
+	            [interpreter<|Interpreter.stack := s|><|Interpreter.gas := gas_after_static|>;
+	             host; tt;
+	             IInterpreterTypes.(InterpreterTypes.InputsTrait_for_Input)
+	               .(InputTraits.target_address) interpreter.(Interpreter.input);
+	             IInterpreterTypes.(InterpreterTypes.RuntimeFlag_for_RuntimeFlag)
+	               .(RuntimeFlag.spec_id) interpreter.(Interpreter.runtime_flag);
+	             tt]%stack).
+	      {
+	        apply Run.PureEq.
+	        cbn.
+	        setoid_rewrite H_static_gas.
+	        cbn.
+	        reflexivity.
+	      }
+	      cbn.
+	      eapply Run.Call
+	        with
+	          (output_inter := false)
+	          (stack_inter :=
+	            [interpreter<|Interpreter.stack := s|><|Interpreter.gas := gas_after_static|>;
+	             host; tt;
+	             IInterpreterTypes.(InterpreterTypes.InputsTrait_for_Input)
+	               .(InputTraits.target_address) interpreter.(Interpreter.input);
+	             IInterpreterTypes.(InterpreterTypes.RuntimeFlag_for_RuntimeFlag)
+	               .(RuntimeFlag.spec_id) interpreter.(Interpreter.runtime_flag);
+	             tt]%stack).
+	      {
+	        apply Run.Pure.
+	      }
+	      cbn.
+	      apply Run.LetUnfold.
+	      cbn.
+	      get_can_access.
+	      cbn.
+	      eapply Run.Call. {
+	        apply Impl_SpecId.is_enabled_in_eq.
+	      }
+	      cbn.
+	      destruct
+	        (Impl_SpecId.is_enabled_in
+	          (IInterpreterTypes.(InterpreterTypes.RuntimeFlag_for_RuntimeFlag)
+	            .(RuntimeFlag.spec_id) interpreter.(Interpreter.runtime_flag))
+	          SpecId.BERLIN) eqn:H_berlin; cbn.
+	      * eapply Run.Call
+	          with
+	            (output_inter := true)
+	            (stack_inter :=
+	              [interpreter<|Interpreter.stack := s|><|Interpreter.gas := gas_after_static|>;
+	               host; tt;
+	               IInterpreterTypes.(InterpreterTypes.InputsTrait_for_Input)
+	                 .(InputTraits.target_address) interpreter.(Interpreter.input);
+	               IInterpreterTypes.(InterpreterTypes.RuntimeFlag_for_RuntimeFlag)
+	                 .(RuntimeFlag.spec_id) interpreter.(Interpreter.runtime_flag);
+	               tt; tt]%stack).
+	        {
+	          apply Run.PureEq.
+	          cbn.
+	          repeat f_equal.
+	        }
+	        cbn.
+	        apply Run.LetUnfold.
+	        cbn.
+	        eapply Run.Call. {
+	          apply Impl_Gas.remaining_interpreter_eq.
+	        }
+	        cbn.
+	        eapply Run.Call. {
+	          apply COLD_SLOAD_COST_ADDITIONAL_eq.
+	        }
+	        cbn.
+	        eapply Run.Call. {
+	          apply Run.Pure.
+	        }
+	        cbn.
+	        apply Run.LetUnfold.
+	        cbn.
+	        get_can_access.
+	        cbn.
+	        get_can_access.
+	        cbn.
+	        eapply Run.Call. {
+	          apply HostEq.
+	        }
+	        destruct
+	          (IHost.(Host.sstore_skip_cold_load) host
+	            (IInterpreterTypes.(InterpreterTypes.InputsTrait_for_Input)
+	              .(InputTraits.target_address) interpreter.(Interpreter.input))
+	            index value
+	            (i[Impl_Gas.remaining gas_after_static] <? (2100 - 100) mod 2 ^ 64))
+	          as [[state_load|load_error] host_after] eqn:H_sstore_result;
+	          cbn.
+	        -- get_can_access.
+	           cbn.
+	           setoid_rewrite H_sstore_result.
+	           cbn.
+	           s. {
+	             apply InterpreterTypesEq.
+	           }
+	           get_can_access.
+	           cbn.
+	           eapply Run.Call. {
+	             apply calc.dyn_sstore_cost_eq.
+	           }
+	           cbn.
+	           s. {
+	             apply Impl_Gas.record_cost_interpreter_eq.
+	           }
+	           match goal with
+	           | |- context[Impl_Gas.record_cost ?gas ?cost] =>
+	               destruct (Impl_Gas.record_cost gas cost)
+	                 as [gas_after_dynamic|] eqn:H_dynamic_gas
+	           end;
+	           cbn.
+	           ++ eapply Run.Call. {
+	                apply Run.Pure.
+	              }
+	              cbn.
+	              eapply Run.Call. {
+	                apply Run.Pure.
+	              }
+	              cbn.
+	              apply Run.LetUnfold.
+	              cbn.
+	              s. {
+	                apply InterpreterTypesEq.
+	              }
+	              eapply Run.Call. {
+	                apply calc.sstore_refund_eq.
+	              }
+	              cbn.
+	              s. {
+	                apply Impl_Gas.record_refund_interpreter_eq.
+	              }
+	              cbn.
+	              apply Run.PureEq.
+	              cbn.
+	              setoid_rewrite H_istanbul.
+	              cbn.
+	              unfold gas_macro.
+	              cbn.
+	              setoid_rewrite H_static_gas.
+	              cbn.
+	              symmetry in H_berlin.
+	              destruct H_berlin.
+	              cbn.
+	              setoid_rewrite H_sstore_result.
+	              cbn.
+	              unfold gas_macro.
+	              cbn.
+	              unfold calc.dyn_sstore_cost in H_dynamic_gas.
+	              unfold calc.sstore_cost in H_dynamic_gas.
+	              cbn in H_dynamic_gas.
+	              unfold calc.dyn_sstore_cost.
+	              unfold calc.sstore_cost.
+	              cbn.
+	              setoid_rewrite H_dynamic_gas.
+	              cbn.
+	              unfold calc.sstore_refund.
+	              cbn.
+	              reflexivity.
+	           ++ s. {
+	                eapply halt_oog_eq;
+	                exact InterpreterTypesEq.
+	              }
+	              cbn.
+	              apply Run.PureEq.
+	              cbn.
+	              setoid_rewrite H_istanbul.
+	              cbn.
+	              unfold gas_macro.
+	              cbn.
+	              setoid_rewrite H_static_gas.
+	              cbn.
+	              symmetry in H_berlin.
+	              destruct H_berlin.
+	              cbn.
+	              setoid_rewrite H_sstore_result.
+	              cbn.
+	              unfold gas_macro.
+	              cbn.
+	              unfold calc.dyn_sstore_cost in H_dynamic_gas.
+	              unfold calc.sstore_cost in H_dynamic_gas.
+	              cbn in H_dynamic_gas.
+	              unfold calc.dyn_sstore_cost.
+	              unfold calc.sstore_cost.
+	              cbn.
+	              setoid_rewrite H_dynamic_gas.
+	              cbn.
+	              reflexivity.
+	        -- destruct load_error; cbn.
+	           ++ get_can_access.
+	              cbn.
+	              setoid_rewrite H_sstore_result.
+	              cbn.
+	              get_can_access.
+	              cbn.
+	              setoid_rewrite H_sstore_result.
+	              cbn.
+	              setoid_rewrite H_sstore_result.
+	              cbn.
+	              s. {
+	                eapply halt_fatal_eq;
+	                exact InterpreterTypesEq.
+	              }
+	              cbn.
+	              apply Run.PureEq.
+	              cbn.
+	              setoid_rewrite H_istanbul.
+	              cbn.
+	              unfold gas_macro.
+	              cbn.
+	              setoid_rewrite H_static_gas.
+	              cbn.
+	              setoid_rewrite H_sstore_result.
+	              cbn.
+	              symmetry in H_berlin.
+	              destruct H_berlin.
+	              cbn.
+	              reflexivity.
+	           ++ get_can_access.
+	              cbn.
+	              setoid_rewrite H_sstore_result.
+	              cbn.
+	              get_can_access.
+	              cbn.
+	              setoid_rewrite H_sstore_result.
+	              cbn.
+	              s. {
+	                eapply halt_oog_eq;
+	                exact InterpreterTypesEq.
+	              }
+	              cbn.
+	              apply Run.PureEq.
+	              cbn.
+	              setoid_rewrite H_istanbul.
+	              cbn.
+	              unfold gas_macro.
+	              cbn.
+	              setoid_rewrite H_static_gas.
+	              cbn.
+	              setoid_rewrite H_sstore_result.
+	              cbn.
+	              symmetry in H_berlin.
+	              destruct H_berlin.
+	              cbn.
+	              reflexivity.
+	      * eapply Run.Call
+	          with
+	            (output_inter := false)
+	            (stack_inter :=
+	              [interpreter<|Interpreter.stack := s|><|Interpreter.gas := gas_after_static|>;
+	               host; tt;
+	               IInterpreterTypes.(InterpreterTypes.InputsTrait_for_Input)
+	                 .(InputTraits.target_address) interpreter.(Interpreter.input);
+	               IInterpreterTypes.(InterpreterTypes.RuntimeFlag_for_RuntimeFlag)
+	                 .(RuntimeFlag.spec_id) interpreter.(Interpreter.runtime_flag);
+	               tt; tt]%stack).
+	        {
+	          apply Run.PureEq.
+	          cbn.
+	          repeat f_equal.
+	        }
+	        cbn.
+	        get_can_access.
+	        cbn.
+	        eapply Run.Call. {
+	          apply HostEq.
+	        }
+	        destruct
+	          (IHost.(Host.sstore) host
+	            (IInterpreterTypes.(InterpreterTypes.InputsTrait_for_Input)
+	              .(InputTraits.target_address) interpreter.(Interpreter.input))
+	            index value)
+	          as [[state_load|] host_after] eqn:H_sstore_result;
+	          cbn.
+	        -- s. {
+	             apply InterpreterTypesEq.
+	           }
+	           get_can_access.
+	           cbn.
+	           eapply Run.Call. {
+	             apply calc.dyn_sstore_cost_eq.
+	           }
+	           cbn.
+	           s. {
+	             apply Impl_Gas.record_cost_interpreter_eq.
+	           }
+	           match goal with
+	           | |- context[Impl_Gas.record_cost ?gas ?cost] =>
+	               destruct (Impl_Gas.record_cost gas cost)
+	                 as [gas_after_dynamic|] eqn:H_dynamic_gas
+	           end;
+	           cbn.
+	           ++ eapply Run.Call. {
+	                apply Run.Pure.
+	              }
+	              cbn.
+	              eapply Run.Call. {
+	                apply Run.Pure.
+	              }
+	              cbn.
+	              apply Run.LetUnfold.
+	              cbn.
+	              s. {
+	                apply InterpreterTypesEq.
+	              }
+	              eapply Run.Call. {
+	                apply calc.sstore_refund_eq.
+	              }
+	              cbn.
+	              s. {
+	                apply Impl_Gas.record_refund_interpreter_eq.
+	              }
+	              cbn.
+	              apply Run.PureEq.
+	              cbn.
+	              setoid_rewrite H_istanbul.
+	              cbn.
+	              unfold gas_macro.
+	              cbn.
+	              setoid_rewrite H_static_gas.
+	              cbn.
+	              symmetry in H_berlin.
+	              destruct H_berlin.
+	              cbn.
+	              setoid_rewrite H_sstore_result.
+	              cbn.
+	              unfold gas_macro.
+	              cbn.
+	              unfold calc.dyn_sstore_cost in H_dynamic_gas.
+	              unfold calc.sstore_cost in H_dynamic_gas.
+	              cbn in H_dynamic_gas.
+	              unfold calc.dyn_sstore_cost.
+	              unfold calc.sstore_cost.
+	              cbn.
+	              setoid_rewrite H_dynamic_gas.
+	              cbn.
+	              unfold calc.sstore_refund.
+	              cbn.
+	              reflexivity.
+	           ++ s. {
+	                eapply halt_oog_eq;
+	                exact InterpreterTypesEq.
+	              }
+	              cbn.
+	              apply Run.PureEq.
+	              cbn.
+	              setoid_rewrite H_istanbul.
+	              cbn.
+	              unfold gas_macro.
+	              cbn.
+	              setoid_rewrite H_static_gas.
+	              cbn.
+	              symmetry in H_berlin.
+	              destruct H_berlin.
+	              cbn.
+	              setoid_rewrite H_sstore_result.
+	              cbn.
+	              unfold gas_macro.
+	              cbn.
+	              unfold calc.dyn_sstore_cost in H_dynamic_gas.
+	              unfold calc.sstore_cost in H_dynamic_gas.
+	              cbn in H_dynamic_gas.
+	              unfold calc.dyn_sstore_cost.
+	              unfold calc.sstore_cost.
+	              cbn.
+	              setoid_rewrite H_dynamic_gas.
+	              cbn.
+	              reflexivity.
+	        -- s. {
+	             eapply halt_fatal_eq;
+	             exact InterpreterTypesEq.
+	           }
+	           cbn.
+	           apply Run.PureEq.
+	           cbn.
+	           setoid_rewrite H_istanbul.
+	           cbn.
+	           unfold gas_macro.
+	           cbn.
+	           setoid_rewrite H_static_gas.
+	           cbn.
+	           symmetry in H_berlin.
+	           destruct H_berlin.
+	           cbn.
+	           setoid_rewrite H_sstore_result.
+	           cbn.
+	           reflexivity.
+	    + eapply Run.Call. {
+	        apply Run.Pure.
+	      }
+	      cbn.
+	      eapply Run.Call. {
+	        apply Run.Pure.
+	      }
+	      cbn.
+	      setoid_rewrite H_static_gas.
+	      cbn.
+	      apply Run.LetUnfold.
+	      cbn.
+	      eapply Run.Call. {
+	        eapply halt_oog_eq;
+	        exact InterpreterTypesEq.
+	      }
+	      cbn.
+	      unfold sstore.
+	      cbn.
+	      setoid_rewrite H_istanbul.
+	      cbn.
+	      unfold gas_macro.
+	      cbn.
+	      apply Run.PureEq.
+	      cbn.
+	      setoid_rewrite H_static_gas.
+	      cbn.
+	      reflexivity.
+Qed.
